Use sandbox for better error messages
Also add some minor utility definitions

PerformanceExperiments/LetIn.v
@@ -3,13 +3,24 @@ Require Import Coq.Setoids.Setoid.
 
 Reserved Notation "'dlet' x .. y := v 'in' f"
          (at level 200, x binder, y binder, f at level 200, format "'dlet'  x .. y  :=  v  'in' '//' f").
+Reserved Notation "'dlet_nd' x .. y := v 'in' f"
+         (at level 200, x binder, y binder, f at level 200, format "'dlet_nd'  x .. y  :=  v  'in' '//' f").
 Definition Let_In {A P} (x : A) (f : forall a : A, P a) : P x := let y := x in f y.
+Definition Let_In_nd {A B} (x : A) (f : A -> B) : B := Let_In x f.
 Notation "'dlet' x .. y := v 'in' f" := (Let_In v (fun x => .. (fun y => f) .. )).
+Notation "'dlet_nd' x .. y := v 'in' f" := (Let_In_nd v (fun x => .. (fun y => f) .. )).
 Strategy 100 [Let_In].
+Strategy 50 [Let_In_nd].
 
 Global Instance Proper_Let_In_nd_changebody {A P R} {Reflexive_R:@Reflexive P R}
   : Proper (eq ==> pointwise_relation _ R ==> R) (@Let_In A (fun _ => P)).
 Proof. lazy; intros; subst; auto; congruence. Qed.
 Global Instance Proper_Let_In_nd_changevalue_forall {A B} {RB:relation B}
   : Proper (eq ==> (forall_relation (fun _ => RB)) ==> RB) (Let_In (P:=fun _:A=>B)).
+Proof. cbv; intuition (subst; eauto). Qed.
+Global Instance Proper_Let_In_nd_nd_changebody {A B R} {Reflexive_R:@Reflexive _ R}
+  : Proper (eq ==> pointwise_relation _ R ==> R) (@Let_In_nd A B).
+Proof. lazy; intros; subst; auto; congruence. Qed.
+Global Instance Proper_Let_In_nd_nd_changevalue_forall {A B} {RB:relation B}
+  : Proper (eq ==> (forall_relation (fun _ => RB)) ==> RB) (@Let_In_nd A B).
 Proof. cbv; intuition (subst; eauto). Qed.
